theories/LambdaWPTactics.v
@@ -709,6 +709,28 @@ Proof using. introv E N. subst. applys Local_erase'. hsimpl~ (``V). Qed.
 
 
 
+Notation "'\forall' x1 , H" := (hforall (fun x1 => H))
+  (at level 39, x1 ident, H at level 50) : heap_scope.
+Notation "'\forall' x1 x2 , H" := (\forall x1, \forall x2, H)
+  (at level 39, x1 ident, x2 ident, H at level 50) : heap_scope.
+Notation "'\forall' x1 x2 x3 , H" := (\forall x1, \forall x2, \forall x3, H)
+  (at level 39, x1 ident, x2 ident, x3 ident, H at level 50) : heap_scope.
+Notation "'\forall' x1 x2 x3 x4 , H" :=
+  (\forall x1, \forall x2, \forall x3, \forall x4, H)
+  (at level 39, x1 ident, x2 ident, x3 ident, x4 ident, H at level 50) : heap_scope.
+Notation "'\forall' x1 x2 x3 x4 x5 , H" :=
+  (\forall x1, \forall x2, \forall x3, \forall x4, \forall x5, H)
+  (at level 39, x1 ident, x2 ident, x3 ident, x4 ident, x5 ident, H at level 50) : heap_scope.
+
+Notation "'\forall' ( x1 : T1 ) , H" := (hforall (fun x1:T1 => H))
+  (at level 39, x1 ident, H at level 50, only parsing) : heap_scope.
+Notation "'\forall' ( x1 : T1 ) ( x2 : T2 ) , H" := (\forall (x1:T1), \forall (x2:T2), H)
+  (at level 39, x1 ident, x2 ident, H at level 50, only parsing) : heap_scope.
+Notation "'\forall' ( x1 : T1 ) ( x2 : T2 ) ( x3 : T3 ) , H" := (\forall (x1:T1), \forall (x2:T2), \forall (x3:T3), H)
+  (at level 39, x1 ident, x2 ident, x3 ident, H at level 50, only parsing) : heap_scope.
+
+
+
 
 
 Definition val_empty : val :=
@@ -731,7 +753,140 @@ Definition Stack `{Enc A} (L:list A) (p:loc) : hprop :=
   p ~~> L.
 
 
-(* todo: why [pat_var "x"] displays with quotes? *)
+Notation "'Case'' t1 '=' p 'Then' t2 'Else' t3" :=
+  (trm_case t1 p t2 t3)
+  (at level 69, t1 at level 0) : trm_scope.
+
+Definition val_test1 : val :=
+  ValFun 'p :=
+    Case' 'p = pat_unit Then 'Fail Else 'Fail.
+
+Definition val_test2 : val :=
+  ValFun 'p :=
+    Case' 'p = 'x Then 'x Else 'Fail.
+
+Notation "'`Case' v1 '=' v2 'Then' F1 'Else' F2" :=
+  (Wp_case_val (fun A EA Q => \[v1 = v2] \-* F1 A EA Q) (v1 <> v2) F2)
+  (at level 69,
+   format "'[v' '`Case'  v1  '='  v2  'Then'  '[' '/' F1 ']' '[' '/'  'Else'  F2 ']' ']'")
+   : charac.
+
+
+Notation "'`Case' v1 '=' v2 [ X1 X2 ] 'Then' F1 'Else' F2" :=
+  (Wp_case_val (fun A EA Q => \forall x1 x2, \[v1 = v2] \-* F1 A EA Q) (forall x1 x2, v1 <> v2) F2)
+  (at level 69,
+   format "'[v' '`Case'  v1  '='  v2  [ X1 X2 ]  'Then'  '[' '/' F1 ']' '[' '/'  'Else'  F2 ']' ']'")
+   : charac.
+
+
+Notation "'`Case'' v1 '=' v2 [ x1 x2 ] 'Then' F1 'Else' F2" :=
+  (Wp_case_val (fun A EA Q => \forall x1 x2, \[v1 = v2] \-* F1 A EA Q) (forall x1 x2, v1 <> v2) F2)
+  (at level 69,
+   format "'[v' '`Case''  v1  '='  v2  [ x1 x2 ]  'Then'  '[' '/' F1 ']' '[' '/'  'Else'  F2 ']' ']'")
+   : charac.
+
+Notation "'`Case' v1 '=' v2 [ x1 ] 'Then' F1 'Else' F2" :=
+  (Wp_case_val (fun A EA Q => \forall x1, \[v1 = v2] \-* F1 A EA Q) (forall x1, v1 <> v2) F2)
+  (at level 69,
+   format "'[v' '`Case'  v1  '='  v2  [ x1 ]  'Then'  '[' '/' F1 ']' '[' '/'  'Else'  F2 ']' ']'")
+   : charac.
+
+
+
+Definition tag_himpl_wp (A:Type) (X:A) := X.
+
+Lemma tag_himpl_wp_intro : forall H F `{EA:Enc A} (Q:A->hprop),
+  tag_himpl_wp (H ==> ^F Q) ->
+  H ==> ^F Q.
+Proof using. auto. Qed.
+
+Notation "'PRE' H 'CODE' F 'POST' Q" := (tag_himpl_wp (H ==> F _ _ Q)) 
+  (at level 67, format "'[v' 'PRE'  H '/' 'CODE'  F '/' 'POST'  Q ']'") : charac.
+
+Ltac tag := applys tag_himpl_wp_intro.
+
+Lemma triple_test2 : forall (p:loc),
+  TRIPLE (val_test2 ``p)
+    PRE \[]
+    POST (fun (u:unit) => \[]).
+Proof using.
+  intros.
+  (* xcf details: *)
+  simpl combiner_to_trm.
+  xcf_prepare_args tt. (* -- not needed here *)
+  let f := xcf_get_fun tt in 
+  unfold f.
+  rew_trms_vals.
+  applys Triple_apps_funs_of_Wp.
+  { reflexivity. }
+  { try xeq_encs. }
+  { reflexivity. }
+  simpl. rew_enc_dyn.
+  unfold Ctx.lookup_or_arbitrary. simpl.
+  unfold Wp_var. simpl.
+  tag.
+Admitted.
+
+
+Lemma triple_test1 : forall (p:loc),
+  TRIPLE (val_test1 ``p)
+    PRE \[]
+    POST (fun (u:unit) => \[]).
+Proof using.
+  intros.
+  (* xcf details: *)
+  simpl combiner_to_trm.
+  xcf_prepare_args tt. (* -- not needed here *)
+  let f := xcf_get_fun tt in 
+  unfold f.
+  rew_trms_vals.
+  applys Triple_apps_funs_of_Wp.
+  { reflexivity. }
+  { try xeq_encs. }
+  { reflexivity. }
+  simpl. rew_enc_dyn.
+  tag.
+Admitted.
+
+Lemma himpl_hand_r : forall H1 H2 H3,
+  H1 ==> H2 ->
+  H1 ==> H3 ->
+  H1 ==> hand H2 H3.
+Proof using. introv M1 M2 Hh. intros b. case_if*. Qed.
+
+Lemma hwand_move_l_pure : forall H1 H2 (P:Prop),
+  (P -> H1 ==> H2) ->
+  H1 ==> (\[P] \-* H2).
+Proof using. introv M. applys hwand_move_l. hsimpl*. Qed.
+
+
+
+Lemma xcase_lemma : forall F1 (P:Prop) F2 H `{EA:Enc A} (Q:A->hprop),
+  (H ==> ^F1 Q) ->
+  (P -> H ==> ^F2 Q) ->
+  H ==> ^(Wp_case_val F1 P F2) Q.
+Proof using. 
+  introv M1 M2. apply Local_erase'. applys himpl_hand_r. 
+  { auto. }
+  { applys* hwand_move_l_pure. }
+Qed.
+
+Lemma xcase_lemma0 : forall F1 (P1 P2:Prop) F2 H `{EA:Enc A} (Q:A->hprop),
+  (P1 -> H ==> ^F1 Q) ->
+  (P2 -> H ==> ^F2 Q) ->
+  H ==> ^(Wp_case_val (fun `{EA1:Enc A1} (Q:A1->hprop) => \[P1] \-* ^F1 Q) P2 F2) Q.
+Proof using. 
+  introv M1 M2. applys* xcase_lemma. { applys* hwand_move_l_pure. }
+Qed.
+
+Lemma xcase_lemma2 : forall (F1:val->val->Formula) (P1:val->val->Prop) (P2:Prop) F2 H `{EA:Enc A} (Q:A->hprop),
+  (forall x1 x2, P1 x1 x2 -> H ==> ^(F1 x1 x2) Q) ->
+  (P2 -> H ==> ^F2 Q) ->
+  H ==> ^(Wp_case_val (fun `{EA1:Enc A1} (Q:A1->hprop) => \forall x1 x2, \[P1 x1 x2] \-* ^(F1 x1 x2) Q) P2 F2) Q.
+Proof using. 
+  introv M1 M2. applys* xcase_lemma.
+  { repeat (applys himpl_hforall_r ;=> ?). applys* hwand_move_l_pure. }
+Qed.
 
 Lemma triple_pop : forall `{Enc A} (p:loc) (L:list A),
   L <> nil ->
@@ -750,13 +905,32 @@ Proof using.
   { reflexivity. }
   { try xeq_encs. }
   { reflexivity. }
-  simpl. rew_enc_dyn. 
-unfold Wp_case_val. simpl.
-unfold Ctx.lookup_or_arbitrary. simpl.
-unfold Wp_var. simpl. unfold fand. simpl.
-(* xcf_post tt. *)
-Admitted.
-
+  simpl; unfold Wp_var; simpl. rew_enc_dyn.
+  tag.
+  (* start *)
+  xunfold Stack.
+  (* xlet *)
+  notypeclasses refine (xlet_instantiate _ _ _ _ _). tag.
+  (* xapp *)
+  applys @xapp_lemma. { eapply @Triple_get. }
+  hsimpl; hsimpl_wand; hsimpl ;=> ? ->. tag.
+  (* xcase *)
+  applys xcase_lemma0 ;=> E1.
+  { destruct L; tryfalse. }
+  { applys xcase_lemma2.
+    2: { intros E. destruct L; rew_enc in *; tryfalse. }
+    { intros x1 x2 E2. destruct L as [|x L']; rew_enc in *; tryfalse.
+      inverts E2.
+      (* xseq *)
+      (* applys xseq_lemma. *)  apply Local_erase'.
+      (* xapp *)
+      applys @xapp_lemma. { applys @Triple_set. }
+      hsimpl; hsimpl_wand. hsimpl.
+      (* xval *)
+     applys~ xval_lemma.
+      (* post *)
+      hsimpl~. } }
+Qed.
 
 Lemma triple_empty : forall `{Enc A} (u:unit),
   TRIPLE (val_empty ``u)
